src/Crypto/Datatypes.dfy
@@ -1,0 +1,6 @@
+// Copyright Amazon.com Inc. or its affiliates. All Rights Reserved.
+// SPDX-License-Identifier: Apache-2.0
+
+module CryptoDatatypes {
+  datatype DigestAlgorithm = SHA_512
+}
